insert_at works

Vector.dfy
@@ -4,14 +4,14 @@ include "NativeInts.dfy"
 class Vector<T>
 {
     var cells: array?<T>;
-    var used: ArrayLength;
+    var length: ArrayLength;
 
     constructor ()
         ensures Valid()
-        ensures this.used == 0
+        ensures this.length == 0
         ensures this.cells == null
     {
-        this.used := 0;
+        this.length := 0;
         this.cells := null;
     }
 
@@ -19,27 +19,30 @@ class Vector<T>
         reads this
     {
         if this.cells == null then
-            this.used == 0
+            this.length == 0
         else (
             (0 < this.cells.Length) &&
             (this.cells.Length <= NativeIntConstants.MaxArrayLengthInt) &&
-            (0 <= used <= cells.Length as ArrayLength)
+            (0 <= length <= cells.Length as ArrayLength)
         )
     }
 
     function method MaxIndex() : (i: ArrayIndex)
-        requires this.used > 0
+        requires this.length > 0
         requires Valid()
         reads this
         ensures i as int < this.cells.Length
     {
-        (this.used - 1) as ArrayIndex
+        (this.length - 1) as ArrayIndex
     }
 
-    function Length() : ArrayLength
+    function method Length() : (l: ArrayLength)
+        requires Valid()
         reads this
+        ensures l == this.length
+        ensures l as int == |this.sequence()|
     {
-        this.used
+        this.length
     }
 
     method try_pop() returns (value: Option<T>)
@@ -47,52 +50,40 @@ class Vector<T>
         modifies this, this.cells
         ensures Valid()
         ensures old(this.cells) == this.cells
-        ensures if old(this.used) > 0 then (
-            (this.used == (old(this.used) - 1)) &&
-            (value == Some(old(this.cells[this.used-1]))) &&
-            (old(this.sequence()[..this.used-1]) == this.sequence()[..this.used])
+        ensures if old(this.length) > 0 then (
+            (this.length == (old(this.length) - 1)) &&
+            (value == Some(old(this.cells[this.length-1]))) &&
+            (old(this.sequence()[..this.length-1]) == this.sequence()[..this.length])
         ) else (
-            (this.used == old(this.used)) &&
+            (this.length == old(this.length)) &&
             (value == None) &&
             (old(this.sequence()) == this.sequence())
         )
     {
-        if (this.cells != null && this.used > 0) {
-            this.used := this.used - 1;
-            return Some(this.cells[this.used]);
+        if (this.cells != null && this.length > 0) {
+            this.length := this.length - 1;
+            return Some(this.cells[this.length]);
         } else {
             return None;
         }
     }
 
-    method alloc(value: T)
-        requires Valid()
-        requires this.cells == null
-        modifies this
-        ensures Valid()
-        ensures old(used) == used
-        ensures this.cells != null && this.cells[..] == [value]
-        ensures fresh(this.cells)
-    {
-        this.cells := new T[1](_ => value);
-    }
-
     method allocOrGrow(value: T)
         requires Valid()
         requires this.cells == null || (
-            this.used as int == this.cells.Length &&
+            this.length as int == this.cells.Length &&
             this.cells.Length < NativeIntConstants.MaxArrayLengthInt
             )
         modifies this
         ensures Valid()
-        ensures old(this.used) == this.used
+        ensures old(this.length) == this.length
         ensures this.cells != null
         ensures fresh(this.cells)
-        ensures old(this.sequence()) == this.sequence()[..this.used]
-        ensures this.cells.Length > this.used as int
+        ensures old(this.sequence()) == this.sequence()[..this.length]
+        ensures this.cells.Length > this.length as int
     {
         if (this.cells == null) {
-            this.alloc(value);
+            this.cells := new T[1](_ => value);
         } else {
             this.grow(value);
         }
@@ -101,11 +92,11 @@ class Vector<T>
     method grow(filler: T)
         requires Valid()
         requires this.cells != null
-        requires this.used as int == this.cells.Length
+        requires this.length as int == this.cells.Length
         requires this.cells.Length < NativeIntConstants.MaxArrayLengthInt
         modifies this
         ensures Valid()
-        ensures old(used) == used
+        ensures old(length) == length
         ensures this.cells != null
         ensures fresh(this.cells)
         ensures this.cells.Length > old(this.cells.Length)
@@ -135,89 +126,96 @@ class Vector<T>
         this.cells := a;
     }
 
+    method {:tailrecursion} bubble_up(idx: ArrayIndex, count: ArrayLength)
+        decreases count
+        requires Valid()
+        requires count >= 2
+        requires idx as int + count  as int <= this.Length() as int
+        modifies this.cells
+        ensures Valid()
+        ensures old(this.sequence()[..idx+1]) == this.sequence()[..idx+1]
+        ensures old(this.sequence()[idx..idx as ArrayLength+count-1]) == this.sequence()[idx+1..idx as ArrayLength+count]
+        ensures old(this.sequence()[idx as ArrayLength+count..]) == this.sequence()[idx as ArrayLength+count..]
+    {
+        ghost var orig_seq := this.sequence();
+        var dst := idx as ArrayLength + count - 1;
+        assert orig_seq[..idx+1] == this.sequence()[..idx+1];
+        this.cells[dst] := this.cells[dst-1];
+        if (count >= 3) {
+            bubble_up(idx, count - 1);
+            assert orig_seq[idx..dst-1] == this.sequence()[idx+1..dst];
+            assert orig_seq[dst-1..dst] == this.sequence()[dst..dst+1];
+            assert orig_seq[idx..dst-1] + orig_seq[dst-1..dst] == orig_seq[idx..dst];
+            assert orig_seq[idx..dst] == this.sequence()[idx+1..dst+1];
+        } else {
+            assert orig_seq[idx..idx as ArrayLength+count-1] == this.sequence()[idx+1..idx as ArrayLength+count];
+        }
+    }
+
     method insert_at(idx: ArrayIndex, value: T)
         requires Valid()
-        requires this.used < NativeIntConstants.MaxArrayLength
+        requires this.length < NativeIntConstants.MaxArrayLength
         requires 0 <= idx as ArrayLength < this.Length()
         modifies this, this.cells
         ensures Valid()
-        ensures this.cells != null
-        ensures (old(this.cells) != this.cells) ==> fresh(this.cells)
-        ensures old(this.used) + 1 == this.used
-        ensures old(this.cells == null) ==> (
-            this.cells.Length == 1 &&
-            this.cells[0] == value
-        )
-        ensures old(this.cells != null) ==> (
-            (old(this.cells.Length) <= this.cells.Length) &&
-            (old(this.cells[..idx]) == this.cells[..idx]) &&
-            (old(this.cells[idx..this.used]) == this.cells[idx+1..this.used])
-        )
-        ensures this.cells[idx] == value
+        ensures old(|this.sequence()|) + 1 == |this.sequence()|
+        ensures old(this.sequence()[..idx]) == this.sequence()[..idx]
+        ensures value == this.sequence()[idx]
+        ensures old(this.sequence()[idx..]) == this.sequence()[idx+1..]
+        ensures old(this.sequence()[..idx] + [value] + this.sequence()[idx..]) == this.sequence()[..]
     {
-        ghost var orig := this.cells[..];
-
-        if (cells == null || used == cells.Length as ArrayLength)
+        if (cells == null || length == cells.Length as ArrayLength)
         {
             this.allocOrGrow(value);
-            assert orig[..idx] == this.cells[..idx];
         }
 
-        assert orig[..idx] == this.cells[..idx];
+        ghost var orig_seq := this.sequence();
 
-        this.used := this.used + 1;
-        var dst := this.MaxIndex();
-        assert idx <= dst;
-        while dst > idx
-            decreases dst as int - idx as int
-            modifies this.cells
-            invariant Valid()
-            invariant this.cells != null
-            invariant orig[..idx] == this.cells[..idx]
-            invariant orig[used..] == this.cells[used..]
-            invariant idx as int <= dst as int < this.used as int <= this.cells.Length
-        {
-            this.cells[dst] := this.cells[dst - 1];
-            dst := dst - 1;
-        }
+        this.length := this.length + 1;
 
-        assert this.cells != null;
-
+        var count := this.length - idx as ArrayLength;
+        assert orig_seq[..idx] == this.sequence()[..idx];
+        bubble_up(idx, count);
+        assert |this.sequence()| == this.length as int;
+        assert this.sequence()[idx+1..] == this.sequence()[idx+1..this.length];
+        assert orig_seq[idx..this.length-1] == this.sequence()[idx+1..this.length];
+        assert orig_seq[idx..this.length-1] == this.sequence()[idx+1..];
         this.cells[idx] := value;
     }
 
     method push(value: T)
         requires Valid()
-        requires this.used < NativeIntConstants.MaxArrayLength
+        requires this.length < NativeIntConstants.MaxArrayLength
         modifies this, this.cells
         ensures Valid()
         ensures this.cells != null
         ensures (old(this.cells) != this.cells) ==> fresh(this.cells)
-        ensures old(this.used) + 1 == this.used
-        ensures old(this.cells == null) || old(this.cells[..this.used]) == this.cells[..(this.used-1)]
-        ensures this.cells[this.used - 1] == value
+        ensures old(this.length) + 1 == this.length
+        ensures old(this.cells == null) || old(this.cells[..this.length]) == this.cells[..(this.length-1)]
+        ensures this.cells[this.length - 1] == value
     {
-        if (cells == null || used == cells.Length as ArrayLength)
+        if (cells == null || length == cells.Length as ArrayLength)
         {
             this.allocOrGrow(value);
         }
 
-        this.cells[used] := value;
-        used := used + 1 as ArrayLength;
+        this.cells[length] := value;
+        length := length + 1 as ArrayLength;
     }
 
     function sequence() : (s: seq<T>)
         requires Valid()
         reads this, this.cells
         ensures |s| <= NativeIntConstants.MaxArrayLengthInt
-        ensures |s| as ArrayLength == this.used
+        ensures |s| as ArrayLength == this.length
+        ensures forall i :: 0 <= i < |s| ==> s[i..] == s[i..this.length]
     {
-        if this.cells == null then [] else this.cells[..this.used]
+        if this.cells == null then [] else this.cells[..this.length]
     }
 
     function method get(i: ArrayIndex) : T
         requires Valid()
-        requires i as ArrayLength < this.used
+        requires i as ArrayLength < this.length
         reads this, this.cells
     {
         this.cells[i]
